\section{The Translation Operator}

\begin{parts}
\item We know that the position operator transforms under the translation operator like so:

  \begin{equation}
    \hat{T}^\dagger(a) \hat{x} \hat{T}(a) = \hat{x} + a.
  \end{equation}

  Acting on both sides with $\hat{T}(a)$ cancels the $\hat{T}^\dagger(a)$ on the left since the translation operator is unitary, so

  \begin{equation}
    \hat{x} \hat{T}(a) = \hat{T}(a)\hat{x} + a\hat{T}(a) \quad\rightarrow \boxed{[\hat{x},\hat{T}(a)] = a\hat{T}(a).}
  \end{equation}


\item We are considering now the how $\braket{\hat{x}}$ and how it compares to $\braket{\hat{x}'}$. First, from the commutator:
  \begin{equation}
    \hat{x}\hat{T}(a) - \hat{T}(a)\hat{x} = a\hat{T}(a).
  \end{equation}
  
  Acting with $\hat{T}^\dagger (a)$:
  
  \begin{equation}
    \hat{T}^\dagger (a)\hat{x}\hat{T}(a) - \hat{x} = a, \quad\rightarrow\quad \hat{x'} = \hat{T}^\dagger(x)\hat{x}\hat{T}(a) = \hat{x} + a.
  \end{equation}

  Thus, 

  \begin{equation}
    \braket{\hat{x}'} = \braket{x | \hat{x} + a | x} = \boxed{\braket{x} + a.}
  \end{equation}
  
\end{parts}

%%% Local Variables:
%%% mode: LaTeX
%%% TeX-master: "../../HW2"
%%% End:
